src/Knapsack/Imlementation/Solution.dfy
@@ -58,7 +58,8 @@ class Solution {
     this.itemsAssign.Length - this.k + 1
   }
 
-
+  //Extends
+  //OptimalExtension
 
 
 }
